some refactoring; add comments

give_up.v
@@ -127,88 +127,229 @@ Section Give_Up_Template.
 
   Definition inFP γ_f n : iProp := ∃ (N: gset Node), own γ_f (◯ N) ∗ ⌜n ∈ N⌝.
 
-  Definition nodePred γ_I γ_k n I_n C_n  :iProp := node n I_n C_n ∗ own γ_k (◯ prod (keyset K I_n n, C_n))
-                                                 ∗ own γ_I (◯ I_n) ∗ ⌜domm I_n = {[n]}⌝.
+  Definition nodePred γ_I γ_k n In Cn  :iProp := 
+                      node n In Cn 
+                    ∗ own γ_k (◯ prod (keyset K In n, Cn))
+                    ∗ own γ_I (◯ In) 
+                    ∗ ⌜domm In = {[n]}⌝.
 
-  Definition CSS (γ_I γ_f γ_k : gname) root (C: gset K) : iProp :=
-    ∃ I, own γ_I (● I) ∗ ⌜globalinv K root I⌝ 
-       ∗ own γ_k (● prod (KS, C))
-       ∗ own γ_f (● domm I) 
-       ∗ ([∗ set] n ∈ (domm I), (∃ (b: bool) (I_n: inset_flowint_ur K),
-            ((lockLoc n) ↦ #b ∗ if b then True 
-                               else (∃ (C_n: gset K), nodePred γ_I γ_k n I_n C_n)))).
+  Definition nodeFull γ_I γ_k n : iProp :=
+    (∃ (b: bool) (In: inset_flowint_ur K),
+        lockLoc n ↦ #b
+        ∗ (if b then True else (∃ Cn, nodePred γ_I γ_k n In Cn))).
+
+  Definition globalGhost γ_I γ_f γ_k r C I : iProp :=
+                    own γ_I (● I) 
+                  ∗ ⌜globalinv K r I⌝ 
+                  ∗ own γ_k (● prod (KS, C))
+                  ∗ own γ_f (● domm I).
+
+  Definition CSSi γ_I γ_f γ_k r C I : iProp :=
+                    globalGhost γ_I γ_f γ_k r C I
+                  ∗ ([∗ set] n ∈ (domm I), nodeFull γ_I γ_k n).
+
+  Definition CSS γ_I γ_f γ_k r C : iProp := ∃ I, CSSi γ_I γ_f γ_k r C I.
     
-  (** High-level lock specs **)
+  (** Some useful lemmas *)
 
-  Lemma lockNode_spec_high (γ_I γ_f γ_k : gname) root n :
-    ⊢ inFP γ_f n -∗ <<< ∀ C, CSS γ_I γ_f γ_k root C >>>
-                             lockNode #n @ ⊤
-                    <<< ∃ I_n C_n, CSS γ_I γ_f γ_k root C ∗ nodePred γ_I γ_k n I_n C_n, RET #() >>>.
+  Lemma inFP_domm γ_I γ_f γ_k r C I n :
+    inFP γ_f n -∗ CSSi γ_I γ_f γ_k r C I -∗ ⌜n ∈ domm I⌝.
   Proof.
-    iIntros "HFp". iIntros (Φ) "AU".
-    awp_apply (lockNode_spec n).
-    iApply (aacc_aupd_commit with "AU"); first done.
-    iIntros (C) "HInv".
-    iDestruct "HInv" as (I) "(H●I & Hglob & H●k & H●f & Hbigstar)".
-    unfold inFP. iDestruct "HFp" as (N0) "(#H◯f & n_in_N)".
-    iDestruct "n_in_N" as %n_in_N.
-    iPoseProof ((auth_own_incl γ_f (domm I) N0) with "[$]") as "%".
-    apply gset_included in H0.
-    assert (n ∈ domm I) as n_in_I by set_solver.
-    rewrite (big_sepS_elem_of_acc _ (domm I) n); last by eauto.
-    iDestruct "Hbigstar" as "(Hn & Hbigstar)".
-    iDestruct "Hn" as (b In) "(Hlock & Hb)".
-    iAaccIntro with "Hlock".
-    { iIntros. iModIntro. iSplitL.
-      iExists I. iFrame "∗". iApply "Hbigstar".
-      iExists b, In. iFrame. iIntros. iModIntro. 
-      iFrame. iExists N0. iFrame "# %". }
-    iIntros "(Hlock & %)". subst b.
-    iModIntro. iDestruct "Hb" as (Cn) "NodePred". 
-    iExists In, Cn. iSplitL.
-    iFrame. iExists I. iFrame. iApply "Hbigstar".
-    iExists true, In. iFrame.
-    iIntros; iModIntro; done.
+    iIntros "#Hfp Hcss".
+    iDestruct "Hcss" as "((HI & Hglob & Hks & Hdom) & Hbigstar)".
+    iDestruct "Hfp" as (N) "(#Hdom' & n_in_N)". iDestruct "n_in_N" as %n_in_N.
+    iPoseProof ((auth_own_incl γ_f (domm I) N) with "[$]") as "#N_incl".
+    iDestruct "N_incl" as %N_incl.
+    apply gset_included in N_incl.
+    iPureIntro. set_solver.
+  Qed.
+
+  Lemma int_domm γ_I γ_f γ_k r C I n In :
+    own γ_I (◯ In) -∗ ⌜domm In = {[n]}⌝ -∗ CSSi γ_I γ_f γ_k r C I -∗ ⌜n ∈ domm I⌝.
+  Proof.
+    iIntros "Hi Dom_In Hcss".
+    iDestruct "Dom_In" as %Dom_In.
+    iDestruct "Hcss" as "((HI & Hglob & Hks & Hdom) & Hbigstar)".
+    iPoseProof ((auth_own_incl γ_I (I) (In)) with "[$]") as "%".
+    rename H0 into I_incl. destruct I_incl as [Io I_incl].
+    iPoseProof (own_valid with "HI") as "%". rename H0 into Valid_I.
+    iPureIntro. rewrite I_incl. rewrite flowint_comp_fp.
+    rewrite Dom_In. set_solver. rewrite <- I_incl.
+    by apply auth_auth_valid. 
   Qed.
   
-  Lemma unlockNode_spec_high (γ_I γ_f γ_k : gname) root n I_n C_n :
-    ⊢ nodePred γ_I γ_k n I_n C_n -∗ <<< ∀ C, CSS γ_I γ_f γ_k root C >>>
-                                              unlockNode #n @ ⊤
-                                      <<< CSS γ_I γ_f γ_k root C, RET #() >>>.
+  Lemma CSS_unfold γ_I γ_f γ_k r C I n :
+    CSSi γ_I γ_f γ_k r C I -∗ ⌜n ∈ domm I⌝ 
+    -∗ (globalGhost γ_I γ_f γ_k r C I ∗ nodeFull γ_I γ_k n
+        ∗ (∀ C',
+           globalGhost γ_I γ_f γ_k r C' I ∗ nodeFull γ_I γ_k n
+           -∗ CSS γ_I γ_f γ_k r C')).
   Proof.
-    iIntros "HN". iIntros (Φ) "AU".
+    iIntros "Hcss %".
+    iDestruct "Hcss" as "((HI & Hglob & Hks & Hdom) & Hbigstar)".
+    rewrite (big_sepS_elem_of_acc _ (domm I) n); last by eauto.
+    iDestruct "Hbigstar" as "(Hn & Hbigstar)". iFrame "∗".
+    iIntros (C') "((HI & Hglob & Hks & Hdom) & H)".
+    iExists I. iFrame "∗". by iApply "Hbigstar".
+  Qed.
+
+  Lemma node_nodeFull_equal γ_I γ_k n In Cn :
+    node n In Cn -∗ nodeFull γ_I γ_k n
+    -∗ (lockLoc n ↦ #true ∗ node n In Cn).
+  Proof.
+    iIntros "Hn Hnf".
+    iDestruct "Hnf" as (b In') "(Hlock & Hnp)". destruct b.
+    - (* Case n locked *)
+      iFrame "∗".
+    - (* Case n unlocked: impossible *)
+      iDestruct "Hnp" as (?C) "(Hn' & _)".
+      iExFalso. iApply (node_sep_star n In In' with "[$]").
+  Qed.
+
+  Lemma CSS_unfold_node_wand γ_I γ_f γ_k r C I n In Cn :
+    CSSi γ_I γ_f γ_k r C I
+    -∗ node n In Cn -∗ ⌜n ∈ domm I⌝
+    -∗ (node n In Cn
+        ∗ globalGhost γ_I γ_f γ_k r C I
+        ∗ lockLoc n ↦ #true
+        ∗ (∀ C',
+           globalGhost γ_I γ_f γ_k r C' I ∗ nodeFull γ_I γ_k n
+           -∗ CSS γ_I γ_f γ_k r C')).
+  Proof.
+    iIntros "Hcssi Hn %".
+    iPoseProof (CSS_unfold with "[$] [%]") as "(Hg & Hnf & Hcss')"; try done.
+    iPoseProof (node_nodeFull_equal with "[$] [$]")
+      as "(Hlock & Hn)".
+    iFrame.
+  Qed.
+
+  Lemma ghost_snapshot_fp γ_f (Ns: gset Node) n:
+    ⊢ own γ_f (● Ns) -∗ ⌜n ∈ Ns⌝ ==∗ own γ_f (● Ns) ∗ inFP γ_f n.
+  Proof.
+    iIntros. 
+    iMod (own_update γ_f (● Ns) (● Ns ⋅ ◯ Ns) with "[$]")
+      as "H".
+    { apply auth_update_core_id. apply gset_core_id. done. }
+    iDestruct "H" as "(Haa & Haf)". iFrame. iModIntro.
+    iExists Ns. by iFrame.
+  Qed.
+
+  (* ghost update for traverse inductive case *)
+  Lemma ghost_update_step γ_I γ_f γ_k r C n In Cn k n' :
+    ⊢ CSS γ_I γ_f γ_k r C
+      -∗ nodePred γ_I γ_k n In Cn
+      -∗ ⌜in_inset K k In n⌝
+      -∗ ⌜in_outset K k In n'⌝
+      ==∗ CSS γ_I γ_f γ_k r C ∗ nodePred γ_I γ_k n In Cn
+      ∗ inFP γ_f n'.
+  Proof.
+    iIntros "Hcss Hnp % %".
+    iDestruct "Hnp" as "(Hn & HkIn & HIn & %)".
+    iDestruct "Hcss" as (I) "Hcssi".
+    iPoseProof (int_domm with "[$] [% //] [$]") as "%".
+    iPoseProof (CSS_unfold_node_wand with "[$] [$] [%]")
+      as "(Hn & Hg & Hlock & Hcss')"; try done.
+    iDestruct "Hg" as "(HI & Hglob & Hks & Hdom)".
+    (* In ≼ I *)
+    iPoseProof ((auth_own_incl γ_I I In) with "[$]")
+      as (Io) "#incl".
+    iDestruct "incl" as %incl. iDestruct "Hglob" as %Hglob.
+    (* Some validities we'll use later *)
+    iPoseProof (own_valid with "HI") as "%".
+    iPoseProof (own_valid with "HIn") as "%".
+    (* Prove the preconditions of ghost_snapshot_fp *)
+    assert (n' ∈ domm Io). 
+    { apply (flowint_step I In Io k n' r); try done. }
+    assert (domm I = domm In ∪ domm Io). {
+      rewrite incl. rewrite flowint_comp_fp. done.
+      rewrite <- incl. by apply auth_auth_valid.
+    }
+    assert (n ∈ domm I). by set_solver.
+    assert (n' ∈ domm I). by set_solver.
+    (* Take snapshot of fp to get inFP n' *)
+    iMod (ghost_snapshot_fp γ_f (domm I) n' with "[$Hdom] [% //]")
+        as "(Hdom & #Hinfp')".
+    iModIntro. iFrame "Hinfp'".
+    iSplitL "Hcss' Hlock HI Hks Hdom". iApply "Hcss'". iFrame "∗ %".
+    iExists true, In. iFrame. iFrame "∗ %".
+  Qed.
+
+  (* root is in footprint *)
+  Lemma ghost_update_root γ_I γ_f γ_k r C :
+    ⊢ CSS γ_I γ_f γ_k r C
+      ==∗ CSS γ_I γ_f γ_k r C ∗ inFP γ_f r.
+  Proof.
+    iIntros "Hcss". 
+    (* Open CSS to get r ∈ domm I *)
+    iDestruct "Hcss" as (I) "((HI & #Hglob & Hks & Hdom) & Hbigstar)".
+    iDestruct "Hglob" as %Hglob.
+    assert (r ∈ domm I)%I as Hroot.
+    { apply globalinv_root_fp. done. }
+    (* Snapshot FP for inFP: *)
+    iMod (ghost_snapshot_fp γ_f (domm I) r with "[$Hdom] [% //]")
+        as "(Hdom & #Hinfp)".
+    iModIntro. iFrame "Hinfp".
+    iExists I. iFrame "∗ %".
+  Qed.
+
+  (** High-level lock specs **)
+
+  Lemma lockNode_spec_high γ_I γ_f γ_k r n :
+    ⊢ inFP γ_f n
+      -∗ <<< ∀ C, CSS γ_I γ_f γ_k r C >>>
+           lockNode #n @ ⊤
+         <<< ∃ In Cn, CSS γ_I γ_f γ_k r C
+                      ∗ nodePred γ_I γ_k n In Cn,
+             RET #() >>>.
+  Proof.
+    iIntros "#HFp". iIntros (Φ) "AU".
+    awp_apply (lockNode_spec n).
+    iApply (aacc_aupd_commit with "AU"); first done.
+    iIntros (C) "Hcss". iDestruct "Hcss" as (I) "Hcssi".
+    iPoseProof (inFP_domm with "[$] [$]") as "%". rename H0 into n_in_I.
+    iPoseProof (CSS_unfold with "[$] [%]") as "(Hg & Hnf & Hcss')"; try done.
+    iSpecialize ("Hcss'" $! C).
+    iDestruct "Hnf" as (b In) "(Hlock & Hnp)".
+    iAaccIntro with "Hlock".
+    { iIntros "Hlockn". iModIntro.
+      iPoseProof ("Hcss'" with "[-]") as "Hcss".
+      { iFrame. iExists b, In. iFrame. }
+      eauto with iFrame.
+    }
+    iIntros "(Hlockn & %)". iModIntro.
+    subst b. iDestruct "Hnp" as (Cn) "Hn".
+    iPoseProof ("Hcss'" with "[-Hn]") as "Hcss".
+    { iFrame. iExists true, In. iFrame. }
+    iExists In, Cn. eauto with iFrame.
+  Qed.
+
+  Lemma unlockNode_spec_high γ_I γ_f γ_k r n In Cn :
+    ⊢ nodePred γ_I γ_k n In Cn
+      -∗ <<< ∀ C, CSS γ_I γ_f γ_k r C >>>
+           unlockNode #n @ ⊤
+         <<< CSS γ_I γ_f γ_k r C, RET #() >>>.
+  Proof.
+    iIntros "Hnp". iIntros (Φ) "AU".
     awp_apply (unlockNode_spec n).
     iApply (aacc_aupd_commit with "AU"); first done.
-    iIntros (C) "HInv".
-    iDestruct "HInv" as (I) "(H●I & Hglob & H●k & H●f & Hbigstar)".
-    iDestruct "HN" as "(Hnode & H◯k & H◯I & Dom_In)".
-    iDestruct "Dom_In" as %Dom_In.
-    iPoseProof ((auth_own_incl γ_I (I) (I_n)) with "[$]") as "%".
-    rename H0 into I_incl. destruct I_incl as [Io I_incl].
-    iPoseProof (own_valid with "H●I") as "%". rename H0 into Valid_I.
-    assert (n ∈ domm I) as n_in_I.
-    { rewrite I_incl. rewrite flowint_comp_fp.
-      rewrite Dom_In. set_solver. rewrite <- I_incl.
-      by apply auth_auth_valid. } 
-    rewrite (big_sepS_elem_of_acc _ (domm I) n); last by eauto.
-    iDestruct "Hbigstar" as "(Hn & Hbigstar)".
-    iDestruct "Hn" as (b In) "(Hlock & Hb)".
-    destruct b; last first.
-    { iDestruct "Hb" as (Cn) "HN'".
-    iDestruct "HN'" as "(Hnode' & _)".
-    iExFalso. iApply node_sep_star.
-    iFrame "Hnode Hnode'". }
+    iIntros (C) "Hcss". iDestruct "Hcss" as (I) "Hcss".
+    iDestruct "Hnp" as "(Hnode & Hk & Hi & Dom_In)".
+    iPoseProof (int_domm with "[$] [$] [$]") as "%".
+    iPoseProof (CSS_unfold_node_wand with "[$] [$] [%]")
+      as "(Hn & Hg & Hlock & Hcss')"; try done.
     iAaccIntro with "Hlock".
-    { iIntros "Hlock". iModIntro. iSplitR "Hnode H◯k H◯I".
-      iExists I. iFrame "∗". iApply "Hbigstar".
-      iExists true, In. iFrame "Hlock". iIntros. iModIntro. 
-      iFrame "∗ %". }
-    iIntros "Hlock". iModIntro. iSplitL.
-    iExists I. iFrame "∗". iApply "Hbigstar".
-    iExists false, I_n. iFrame.
-    iExists C_n. iFrame "∗ # %".
-    iIntros; iModIntro; done.
-  Qed.
+    { iIntros "Hlock". iModIntro.
+      iPoseProof ("Hcss'" with "[-Hn Hk Hi Dom_In]") as "Hcss".
+      { iFrame. iExists true, In. iFrame. }
+      iFrame "Hcss". iIntros "AU". iModIntro.
+      iSplitR "AU". iFrame "∗ #". done.
+    }
+    iIntros "Hlock". iModIntro.
+    iPoseProof ("Hcss'" with "[-]") as "Hcss".
+    { iFrame. iExists false, In. iFrame. iExists Cn. iFrame "∗ #". }
+    eauto with iFrame.
+ Qed.
+
 
   (** Proofs of traverse and CSSOp *)
 
@@ -224,164 +365,145 @@ Section Give_Up_Template.
     iLöb as "IH" forall (n). iIntros "(#Hks & #Hfp)".
     iDestruct "Hks" as %k_in_KS.
     iIntros (Φ) "AU". wp_lam. wp_let. wp_bind(lockNode _)%E.
+    (* Open AU to get lockNode precondition *)
     awp_apply (lockNode_spec_high γ_I γ_f γ_k root n); try done.
     iApply (aacc_aupd_abort with "AU"); first done.
     iIntros (C0) "HInv". iAaccIntro with "HInv".
     { iIntros "HInv". iModIntro. eauto with iFrame. }
     iIntros (In Cn) "(HInv & Nodepred)".
+    (* Close AU and move on *)
     iModIntro. iFrame. iIntros "AU". iModIntro.
     wp_pures. wp_bind (inRange _ _)%E.
     iDestruct "Nodepred" as "(Hnode & H◯k & H◯I & Dom_In)".
-    iApply fupd_wp. iMod "AU" as (C1) "[HInv [Hclose _]]".
-    iDestruct "HInv" as (I) "(H●I & Hglob & H●k & H●f & Hbigstar)".
-    iDestruct "Dom_In" as %Dom_In.
-    iPoseProof ((auth_own_incl γ_I (I) (In)) with "[$]") as "%".
-    rename H0 into I_incl. destruct I_incl as [Io I_incl].
-    iPoseProof (own_valid with "H●I") as "%". rename H0 into Valid_I.
-    iDestruct "Hglob" as %Hglob.
-    iMod (own_update γ_f (● (domm I)) (● (domm I) ⋅ ◯ (domm I)) with "H●f") as "H".
-    apply auth_update_core_id. apply gset_core_id. done.
-    iDestruct "H" as "(H●f & #H◯_dommI)".
-    iMod ("Hclose" with "[H●I H●k H●f Hbigstar]") as "AU".
-    iExists I. iFrame "∗ %". iModIntro.    
     wp_apply ((inRange_spec n k In Cn) with "Hnode").
     iIntros (b) "(Hnode & Hb)". destruct b.
-    - wp_pures. wp_bind (findNext _ _)%E. iSimpl in "Hb".
+    - (* Case : inRange returns true *)
+      wp_pures. wp_bind (findNext _ _)%E. iSimpl in "Hb".
       iDestruct "Hb" as %Hinset. specialize (Hinset Coq.Init.Logic.I).
       wp_apply ((findNext_spec n k In Cn) with "[Hnode]"). iFrame "∗ %".
       iIntros (b n') "(Hnode & Hbb)". destruct b.
-      + wp_pures. iDestruct "Hbb" as %in_outset.  
-        awp_apply ((unlockNode_spec_high γ_I γ_f γ_k root n) with "[-AU]").
-        iFrame "∗ %". iApply (aacc_aupd_abort with "AU"); first done.
+      + (* Case : findNext returns Some n' *)
+        wp_pures. iDestruct "Hbb" as %in_outset.
+        (* Get CSS from AU to step to n' *)
+        iApply fupd_wp. iMod "AU" as (C) "[Hcss [Hclose _]]".
+        iAssert (nodePred γ_I γ_k n In Cn)%I 
+                        with "[H◯k H◯I Dom_In Hnode]" as "Hn". by iFrame.
+        (* ghost update to step to n' *)                
+        iMod (ghost_update_step with "[$] [$] [% //] [% //]") as "(Hcss & Hnp & #Hinfp')".
+        (* Close AU *)
+        iMod ("Hclose" with "Hcss") as "AU". iModIntro.
+        (* Unlock node n *)
+        awp_apply ((unlockNode_spec_high γ_I γ_f γ_k root n) with "[-AU //]").
+        iApply (aacc_aupd_abort with "AU"); first done.
         iIntros (C2) "HInv". iAaccIntro with "HInv".
         { iIntros "HInv". iModIntro. eauto with iFrame. }
         iIntros "HInv". iModIntro. iFrame. iIntros "AU".
-        iModIntro. wp_pures. iApply "IH"; try done. iFrame "%".
-        iExists (domm I). iFrame "#". iPureIntro.
-        assert (n' ∈ domm Io).
-        { apply (flowint_step I In Io k n' root); try done. }
-        rewrite I_incl. rewrite intComp_dom. set_solver.
-        rewrite <-I_incl. by apply auth_auth_valid.     
-      + iDestruct "Hbb" as %not_in_outset.
+        iModIntro. wp_pures.
+        (* Apply induction hypothesis on n' *) 
+        iApply "IH"; try done. iFrame "% #".
+      + (* Case : findNext returns None *)
+        iDestruct "Hbb" as %not_in_outset.
+        (* Open AU and commit *)
         iApply fupd_wp. iMod "AU" as (C) "[HInv [_ Hclose]]".
         iSpecialize ("Hclose" $! n In Cn).
+        iDestruct "Dom_In" as "%".
         iMod ("Hclose" with "[H◯k H◯I HInv Hnode]").
         iFrame "∗ # %". iModIntro. wp_pures. done.
-    - wp_pures. iDestruct "Hb" as %Hnot_in_inset.
+    - (* Case : inRange returns false *)
+      wp_pures. iDestruct "Hb" as %Hnot_in_inset.
+      (* Unlock node n *)
       awp_apply ((unlockNode_spec_high γ_I γ_f γ_k root n) with "[-AU]").
       iFrame "∗ # %". iApply (aacc_aupd_abort with "AU"); first done.
       iIntros (C) "HInv". iAaccIntro with "HInv".
       { iIntros. iModIntro. eauto with iFrame. }
-      iIntros "HInv". iModIntro. iFrame. iIntros "AU".
-      iModIntro. wp_pures. iApply "IH"; try done. iFrame "%".
-      iExists (domm I). iFrame "H◯_dommI". iPureIntro.
-      unfold globalinv in Hglob. by destruct Hglob as (_ & Hglob & _).
+      iIntros "HInv".
+      (* Get pre of inductive hypothesis with root before closing AU *)
+      iMod (ghost_update_root with "[$]") as "(HInv & #HinFPr)".
+      iModIntro. iFrame. iIntros "AU".
+      iModIntro. wp_pures.
+      (* Apply induction hypothesis on root *)
+      iApply "IH"; try done. iFrame "% #".
   Qed.
 
   (** Verification of abstract specification of the search structure operation. *)
   
-  (*Instance Ψ_persistent dop (k : K) C C' res : Persistent (Ψ dop k C C' res : iProp).
-  Proof. destruct dop; apply _. Qed.*)
-
   Theorem CSSOp_spec (γ_I γ_f γ_k: gname) root (dop: dOp) (k: K):
    ⊢ ⌜k ∈ KS⌝ -∗ <<< ∀ C, CSS γ_I γ_f γ_k root C >>>
-      CSSOp dop root #k @ ⊤
-    <<< ∃ C' (res: bool), CSS γ_I γ_f γ_k root C'
-        ∗ (Ψ dop k C C' res : iProp), RET #res >>>.
+                          CSSOp dop root #k @ ⊤
+                 <<< ∃ C' (res: bool), CSS γ_I γ_f γ_k root C'
+                                     ∗ (Ψ dop k C C' res : iProp), RET #res >>>.
   Proof.
     iIntros "HKin" (Φ) "AU". iLöb as "IH". wp_lam.
     iDestruct "HKin" as %k_in_KS.
+    (* Open AU and get pre for traverse_spec *)
     iApply fupd_wp. iMod "AU" as (C0) "[HInv [HAU _]]".
-    iDestruct "HInv" as (I0) "(H●I & Hglob & H●k & H●f & Hbigstar)".
-    iMod (own_update γ_f (● (domm I0)) (● (domm I0) ⋅ ◯ (domm I0)) with "H●f") as "H".
-    apply auth_update_core_id. apply gset_core_id. done.
-    iDestruct "H" as "(H●f & #H◯domm)". iDestruct "Hglob" as %Hglob.
-    iMod ("HAU" with "[-IH]") as "AU". iExists I0. iFrame "∗ # %".
-    iModIntro. wp_bind (traverse _ _ _)%E.
-    awp_apply (traverse_spec γ_I γ_f γ_k k root root).
-    { iFrame "%". iExists (domm I0). iFrame "#". iPureIntro.
-    unfold globalinv in Hglob. by destruct Hglob as (_ & Hglob & _). }
+    iMod (ghost_update_root with "[$]") as "(HInv & #HinFPr)".
+    (* Close AU *)
+    iMod ("HAU" with "HInv") as "AU". iModIntro.
+    (* Open AU and apply traverse_spec *)
+    awp_apply (traverse_spec γ_I γ_f γ_k k root root); first by iFrame "% #".
     iApply (aacc_aupd_abort with "AU"); first done.
     iIntros (C1) "HInv". iAaccIntro with "HInv"; first by eauto with iFrame.
+    (* traverse returns node n and it's local ghost state *)
     iIntros (n In Cn) "(HInv & Nodepred & % & %)".
-    rename H0 into in_inset. rename H1 into not_in_outset. 
+    rename H0 into in_inset. rename H1 into not_in_outset.
+    (* Close AU and move on *) 
     iModIntro. iFrame. iIntros "AU".
     iModIntro. wp_pures. wp_bind (decisiveOp _ _ _)%E.
-    iDestruct "Nodepred" as "(Hnode & H◯k & H◯I & Dom_In)".
+    iDestruct "Nodepred" as "(Hnode & Hk & Hi & Dom_In)".
     wp_apply ((decisiveOp_spec dop n k In Cn) with "[Hnode]"). eauto with iFrame.
     iIntros (b res Cn'). iIntros "(Hnode & Hb)". destruct b.
-    - iDestruct "Hb" as "#HΨ".
+    - (* Case : decisiveOp succeeds *)
+      iDestruct "Hb" as "#HΨ".
       wp_pures. wp_bind(unlockNode _)%E.
+      (* Note: cannot use unlockNode_spec_high here because 
+         that needs nodePred, which we won't have until we linearize,
+         which we can't do until we open the AU.
+         We can't open the AU before unlockNode, because linearizing will
+         mean committing the AU and giving up CSS (needed by unlockNode).
+         So we manually execute unlockNode_spec and linearize simultaneously.
+       *)      
       awp_apply (unlockNode_spec n).
-      iApply (aacc_aupd_commit with "AU"); first done. iIntros (C2) "HInv".
-      iDestruct "HInv" as (I2) "(H●I & Hglob & H●k & H●f & Hbigstar)".
-      iDestruct "Dom_In" as %Dom_In.
-      iPoseProof ((auth_own_incl γ_I (I2) (In)) with "[$]") as "%".
-     rename H0 into I_incl. destruct I_incl as [Io I_incl].
-      iPoseProof (own_valid with "H●I") as "%". rename H0 into Valid_I.
-      assert (n ∈ domm I2) as n_in_I2.
-      { rewrite I_incl. rewrite flowint_comp_fp.
-        rewrite Dom_In. set_solver. rewrite <- I_incl.
-        by apply auth_auth_valid. } 
-      rewrite (big_sepS_elem_of_acc _ (domm I2) n); last by eauto.
-      iDestruct "Hbigstar" as "(Hn & Hbigstar)".
-      iDestruct "Hn" as (b In') "(Hlock & Hb)".
-      destruct b; last first.
-      { iDestruct "Hb" as (Cn'') "HN'".
-      iDestruct "HN'" as "(Hnode' & _)".
-      iExFalso. iApply node_sep_star.
-      iFrame "Hnode Hnode'". }
+      iApply (aacc_aupd_commit with "AU"); first done.
+      iIntros (C2) "HInv". iDestruct "HInv" as (I2)"HInv".
+      (* Unfold CSS to execute unlockNode *)
+      iPoseProof (int_domm with "[$] [$] [$]") as "%".      
+      iPoseProof (CSS_unfold_node_wand with "[$] [$] [%]")
+        as "(Hn & Hg & Hlock & Hcss')"; try done.
       iAaccIntro with "Hlock".
-      { iIntros "Hlock". iModIntro. iSplitR "Hnode H◯k H◯I".
-        iExists I2. iFrame "∗". iApply "Hbigstar".
-        iExists true, In. iFrame "Hlock". iIntros. iModIntro. 
-        iFrame "∗ %". }
+      { iIntros "Hlock". iModIntro.
+        iPoseProof ("Hcss'" with "[-Hn Hk Hi Dom_In]") as "Hcss".
+        { iFrame. iExists true, In. iFrame. }
+        iFrame "Hcss". iIntros "AU". iModIntro. iFrame.
+      }
       iIntros "Hlock".
-      iPoseProof (own_valid with "H◯I") as "%". rename H0 into Hvldn. 
-      iPoseProof (own_valid with "H◯k") as "%". rename H0 into HvldCn.
-      rewrite auth_frag_valid in HvldCn *; intros HvldCn. unfold valid, cmra_valid in HvldCn.
-      simpl in HvldCn. unfold ucmra_valid in HvldCn. simpl in HvldCn.
-      iMod ((ghost_update_keyset γ_k dop k Cn Cn' res (keyset K In n) C2) with "[H●k H◯k]") as "Hgks".
-      assert (k ∈ keyset K In n) as K_in_ksIn. apply keyset_def; try done.
-      iFrame "% ∗ #". iEval (unfold Ψ) in "HΨ".
-      { destruct dop.
-        - iDestruct "HΨ" as %(HΨ & _). iPureIntro. subst Cn'. done.
-        - iDestruct "HΨ" as %(HΨ & _). iPureIntro. set_solver.
-        - iDestruct "HΨ" as %(HΨ & _). iPureIntro. set_solver. }
-      iDestruct "Hgks" as (C2') "(#HΨC & H●k & H◯k)".
-      iModIntro. iExists (C2'), res. iSplitL. iFrame "HΨC".
-      iExists I2. iFrame "∗ % #". iApply "Hbigstar". iExists false, In. iFrame "∗ # %".
+      (* Commit AU *)
+      iDestruct "Hg" as "(HI & Hglob & Hks & Hdom)".
+      iMod ((ghost_update_keyset γ_k dop k Cn Cn' res (keyset K In n) C2)
+              with "[Hk Hks]") as (C2') "(#HΨC & Hks & HkIn)".
+      {
+        iPoseProof (keyset_valid with "Hk") as "%".
+        assert (k ∈ keyset K In n); first by apply keyset_def.
+        iPoseProof ((Ψ_impl_C_in_K _ _ _ _ _ (keyset K In n))
+                      with "[$HΨ] [% //] [% //]") as "%".
+        iFrame "∗ #". by iPureIntro.
+      }
+      iModIntro.
+      (* Close AU *)
+      iExists C2', res. iSplitL. iFrame "HΨC".
+      iApply "Hcss'". iFrame "∗ % #". iExists false, In. iFrame "∗ # %".
       iExists Cn'. iFrame. iIntros. iModIntro. by wp_pures. 
-    - wp_match. awp_apply (unlockNode_spec n).
-      iApply (aacc_aupd_abort with "AU"); first done. iIntros (C2) "HInv".
-      iDestruct "HInv" as (I1) "(H●I & Hglob & H●k & H●f & Hbigstar)".
-      iDestruct "Dom_In" as %Dom_In.
-      iPoseProof ((auth_own_incl γ_I (I1) (In)) with "[$]") as "%".
-     rename H0 into I_incl. destruct I_incl as [Io I_incl].
-      iPoseProof (own_valid with "H●I") as "%". rename H0 into Valid_I.
-      assert (n ∈ domm I1) as n_in_I1.
-      { rewrite I_incl. rewrite flowint_comp_fp.
-        rewrite Dom_In. set_solver. rewrite <- I_incl.
-        by apply auth_auth_valid. } 
-      rewrite (big_sepS_elem_of_acc _ (domm I1) n); last by eauto.
-      iDestruct "Hbigstar" as "(Hn & Hbigstar)".
-      iDestruct "Hn" as (b In') "(Hlock & HN)".
-      destruct b; last first.
-      { iDestruct "HN" as (Cn'') "HN'".
-      iDestruct "HN'" as "(Hnode' & _)".
-      iExFalso. iApply node_sep_star.
-      iFrame "Hnode Hnode'". }
-      iDestruct "Hb" as %Hb.
-      iAaccIntro with "Hlock".
-      { iIntros "Hlock". iModIntro. iSplitR "Hnode H◯k H◯I".
-        iExists I1. iFrame "∗". iApply "Hbigstar".
-        iExists true, In. iFrame "Hlock". iIntros. iModIntro. 
-        iFrame "∗ %". }
-      iIntros "Hlock". iModIntro. iSplitL.
-      iExists I1. iFrame. iApply "Hbigstar".
-      iExists false, In. iFrame. iExists Cn.
-      replace Cn'. iFrame "∗ % #".
-      iIntros "AU". iModIntro. wp_pures.
+    - (* Case : decisiveOp fails *) 
+      wp_match. iDestruct "Hb" as "%". subst Cn'.
+      (* Open AU and apply unlockNode spec *)
+      awp_apply ((unlockNode_spec_high γ_I γ_f γ_k root n) with "[-AU]").
+      iFrame. iApply (aacc_aupd_abort with "AU"); first done.
+      iIntros (C2) "HInv".
+      (* execute unlockNode and close AU *)
+      iAaccIntro with "HInv"; try 
+        iIntros "HInv"; iModIntro; iFrame; iIntros; iModIntro; try done.     
+      wp_pures.
+      (* Apply induction hypothesis *)
       iApply "IH"; try done.
   Qed.      
 
